NatNormalForm/Relation.lean
@@ -1,0 +1,762 @@
+axiom prop_retractible: forall {P: Prop} {x y: P}, x = y
+
+/-!
+# Relations
+
+A relation is just a binary predicate over some type
+-/
+
+abbrev Relation (A: Type) := A -> A -> Prop
+
+class Reflexive {A: Type} (P: Relation A) where
+  refl: forall {a: A}, P a a
+
+def Relation.refl {A: Type} {P: Relation A} [inst: Reflexive P]:
+  forall {a: A}, P a a := inst.refl
+
+
+class Antisymmetric {A: Type} (P: Relation A) where
+  anti: forall {a b: A}, P a b -> P b a -> a = b
+
+def Relation.anti {A: Type} {P: Relation A} [inst: Antisymmetric P]:
+  forall {a b: A}, P a b -> P b a -> a = b := inst.anti
+
+
+class Transitive {A: Type} (P: Relation A) where
+  trans: forall {a b c: A}, P a b -> P b c -> P a c
+
+def Relation.trans {A: Type} {P: Relation A} [inst: Transitive P]:
+  forall {a b c: A}, P a b -> P b c -> P a c := inst.trans
+
+
+class Symmetric {A: Type} (P: Relation A) where
+  symm: forall {a b: A}, P a b -> P b a
+
+def Relation.symm {A: Type} {P: Relation A} [inst: Symmetric P]:
+  forall {a b: A}, P a b -> P b a := inst.symm
+
+
+inductive Fold {A: Type} (P: Relation A): Nat -> Relation A where
+  | zero {a}: Fold P 0 a a
+  | succ {n a b c}: Fold P n a b -> P b c -> Fold P (n+1) a c
+
+
+inductive Inverse {A} (P: Relation A): Relation A where
+  | inv {a b}: P a b -> Inverse P b a
+
+
+def Relation.inv {A a b} (P: Relation A): P a b -> Inverse P b a:= Inverse.inv
+
+
+class Congruence {A: Type} (P: Relation A) (S: A -> A) where
+  rel_cong: forall {a b: A}, (P a b) -> P (S a) (S b)
+
+
+class KeepCong {A: Type} (P Q: Relation A) where
+  keep_cong: forall (f: A -> A),
+    (forall {a b}, (P a b) -> P (f a) (f b)) ->
+    forall {a b}, (Q a b) -> Q (f a) (f b)
+
+
+def Relation.keep_cong {A: Type}
+  {P Q: Relation A} (f: A -> A)
+  [inst: KeepCong P Q]:
+    (forall {a b}, (P a b) -> P (f a) (f b)) ->
+    forall {a b}, (Q a b) -> Q (f a) (f b) :=
+    inst.keep_cong f
+
+
+/--
+The defintion of a sub relation
+-/
+class SubRel {A} (P: Relation A) (Q: Relation A): Prop where
+  inclusion: forall {a b: A}, P a b -> Q a b
+
+notation: 60 P " sub_rel " Q => SubRel P Q
+
+def Relation.inclusion {A: Type} {P: Relation A} {Super: Relation A}
+  [inst: P sub_rel Super]: forall {a b: A}, P a b -> Super a b :=
+    inst.inclusion
+
+/-!
+`SubRel` is it self a poset on all relations
+-/
+section
+
+instance sub_rel_refl {A: Type} {P: Relation A}: P sub_rel P where
+  inclusion := id
+
+instance: forall {A: Type}, Reflexive (SubRel (A := A)) where
+  refl := by
+    intros P
+    apply sub_rel_refl
+
+
+instance: forall {A: Type}, Transitive (SubRel (A := A)) where
+  trans {P Q R} {s1 s2} := by
+    apply SubRel.mk
+    intros a b H
+    apply Q.inclusion
+    apply P.inclusion
+    apply H
+
+
+theorem sub_rel_equiv: forall {A: Type} {P Q: Relation A},
+  (P sub_rel Q) -> (Q sub_rel P) -> forall {a b: A}, P a b <-> Q a b := by
+  intros A P Q s1 s2
+  intros a b
+  constructor
+  . apply s1.inclusion
+  . apply s2.inclusion
+
+theorem rel_eq: forall {A: Type} {P Q: Relation A}, (forall x y: A, P x y <-> Q x y) -> P = Q := by
+  intros A P Q H
+  apply funext
+  intros x
+  apply funext
+  intros y
+  apply propext
+  apply H
+
+instance: forall {A: Type}, Antisymmetric (SubRel (A := A)) where
+  anti := by
+    intros P Q s1 s2
+    apply rel_eq
+    intros a b
+    apply Iff.intro
+    . apply s1.inclusion
+    . apply s2.inclusion
+end
+
+
+/-!
+The next thing is to prove what is a closure.
+-/
+section Closure
+
+abbrev RelationOp (A: Type) := Relation A -> Relation A
+abbrev RelationPred (A: Type) := Relation A -> Prop
+
+/-!
+The closure fo each type is clear.
+-/
+class Closure {A: Type} (Pred: outParam (RelationPred A)) (P: outParam (Relation A)) (C: Relation A) where
+  sub: P sub_rel C
+  pred: Pred C
+  least: forall {Q: Relation A}, Pred Q -> (P sub_rel Q) -> C sub_rel Q
+
+
+/-!
+We instantly have the following.
+-/
+instance {A: Type} {P C: Relation A} {Pred: RelationPred A} [inst: Closure Pred P C]:
+  P sub_rel C := inst.sub
+
+instance cl_cl_sub {A: Type} {Pred: RelationPred A} {P: Relation A} {C1 C2: Relation A}
+  [inst1: Closure Pred P C1] [inst2: Closure Pred P C2]: C1 sub_rel C2 where
+    inclusion := by
+      intros a b
+      let sub := @inst1.least C2 inst2.pred inst2.sub
+      apply sub.inclusion
+
+
+theorem cl_unique: forall {A: Type} {Pred: RelationPred A} {P: Relation A} {C1 C2: Relation A}
+  [Closure Pred P C1] [Closure Pred P C2], C1 = C2 := by
+  intros A Pred P C1 C2 inst1 inst2
+  apply rel_eq
+  apply sub_rel_equiv
+  . /- C1 sub_rel C2 -/
+    apply @cl_cl_sub A Pred P C1 C2 inst1 inst2
+  . /- C2 sub_rel C1 -/
+    apply @cl_cl_sub A Pred P C2 C1 inst2 inst1
+
+/-!
+We can also define a closure operator.
+-/
+class ClosureOp {A: Type} (Pred: outParam (RelationPred A)) (Cl: outParam (RelationOp A)) where
+  close (P: Relation A): Closure Pred P (Cl P)
+  closed {P: Relation A} := close P
+  sub {P: Relation A} := closed.sub (P := P)
+  pred {P: Relation A} := closed.pred (P := P)
+  least {P Q: Relation A} := closed.least (P := P) (Q := Q)
+
+
+def RelationOp.close {A: Type} (Cl: RelationOp A) (P: Relation A) {Pred: RelationPred A}
+  [inst: ClosureOp Pred Cl] := inst.close P
+
+def RelationOp.closed {A: Type} (Cl: RelationOp A) {P: Relation A} {Pred: RelationPred A}
+  [inst: ClosureOp Pred Cl] := inst.close P
+
+/-!
+Then, the `Closure` instances are defined as follows.
+-/
+instance {A: Type} {Pred: RelationPred A} (Cl: RelationOp A) [inst: ClosureOp Pred Cl]
+  (P: Relation A): Closure Pred P (Cl P) := inst.closed
+
+
+instance {A: Type} {Pred: RelationPred A} {Cl: RelationOp A} [inst: ClosureOp Pred Cl] {P: Relation A}:
+  P sub_rel (Cl P) := (inst.closed).sub
+
+instance cl_op_cl_op_sub {A: Type} {Pred: RelationPred A} {C1 C2: RelationOp A}
+  [inst1: ClosureOp Pred C1] [inst2: ClosureOp Pred C2] {P: Relation A}: C1 P sub_rel C2 P where
+    inclusion := by
+      intros a b
+      let sub := @inst1.least P (C2 P) inst2.pred inst2.sub
+      apply sub.inclusion
+
+instance cl_mono {A: Type} {Pred: RelationPred A} {Cl: RelationOp A} [inst: ClosureOp Pred Cl]
+  {P Q: Relation A} [r1: P sub_rel Q]: Cl P sub_rel Cl Q where
+  inclusion := by
+    have r2: Q sub_rel Cl Q := inst.sub
+    have r3: P sub_rel Cl Q := Relation.trans r1 r2
+    let H := @inst.least P (Cl Q) inst.pred r3
+    intros a b
+    apply H.inclusion
+
+theorem rel_op_eq: forall {A: Type} {C1 C2: RelationOp A},
+  (forall {P: Relation A}, C1 P = C2 P) -> C1 = C2 := by
+  intros A C1 C2 H
+  apply funext
+  apply H
+
+theorem cl_op_unique: forall {A: Type} {Pred: RelationPred A} (C1 C2: RelationOp A),
+  [ClosureOp Pred C1] -> [ClosureOp Pred C2] -> C1 = C2 := by
+  intros A pred C1 C2 inst1 inst2
+  apply rel_op_eq
+  intros P
+  apply rel_eq
+  apply sub_rel_equiv
+  . apply @cl_op_cl_op_sub A pred C1 C2 inst1 inst2
+  . apply @cl_op_cl_op_sub A pred C2 C1 inst2 inst1
+
+/-!
+Then, it is reasonable to define the following.
+-/
+
+def Relation.closed {A: Type} {Pred: RelationPred A} {Cl: RelationOp A} [inst: ClosureOp Pred Cl]
+  {P: Relation A} := inst.close P
+
+def Relation.pred {A: Type} {Pred: RelationPred A} {Cl: RelationOp A} [inst: ClosureOp Pred Cl]
+  {P: Relation A}: Pred (Cl P) := inst.pred
+
+def Relation.least {A: Type} {Pred: RelationPred A} (Cl: RelationOp A) [inst: ClosureOp Pred Cl]
+  {P: Relation A}: forall {Q: Relation A}, Pred Q -> (P sub_rel Q) -> (Cl P sub_rel Q) := inst.least
+
+
+/-!
+We are going to deal with a closure `Cl` with respect to `Pred`
+-/
+variable {A: Type}
+variable {P: Relation A}
+variable {Pred: RelationPred A}
+variable {Cl: RelationOp A}
+variable [inst: ClosureOp Pred Cl]
+
+instance cl_cl_sub_cl: Cl (Cl P) sub_rel (Cl P) := inst.least (P := Cl P) (Q := Cl P) inst.pred Relation.refl
+
+theorem cl_cl_is_cl {Cl: RelationOp A} [inst: ClosureOp Pred Cl]: Cl (Cl P) = Cl P := by
+  apply rel_eq
+  apply sub_rel_equiv
+  . apply cl_cl_sub_cl
+  . apply @inst.sub
+end Closure
+
+
+/---
+Reflexive closure
+-/
+inductive RCl {A} (P: Relation A): Relation A where
+  | inclusion {a b}: P a b -> RCl P a b
+  | refl {a}: RCl P a a
+
+instance RCl.close {A: Type} (P: Relation A): Closure Reflexive P (RCl P) where
+  sub := SubRel.mk RCl.inclusion
+  pred := Reflexive.mk RCl.refl
+  least := by
+    intros Q inst sub
+    apply SubRel.mk
+    intros a b H
+    cases H
+    case inclusion Hab =>
+      apply P.inclusion
+      apply Hab
+    case refl => apply inst.refl
+
+
+instance {A: Type}: ClosureOp Reflexive (RCl (A := A)) where
+  close := RCl.close
+
+instance: Reflexive (RCl P) where
+  refl := RCl.refl
+
+
+theorem rcl_ab_or_eq {A: Type} {P: Relation A}:
+  forall {a b: A}, RCl P a b -> P a b ∨ a = b := by
+  intros a b H
+  induction H
+  case inclusion a b Hab =>
+    left
+    apply Hab
+  case refl a =>
+    right
+    rfl
+
+
+/--
+Transitive closure
+-/
+inductive TCl {A} (P: Relation A): Relation A where
+  | inclusion {a b}: P a b -> TCl P a b
+  | trans {a b c}: TCl P a b -> TCl P b c -> TCl P a c
+
+instance TCl.close {A: Type} (P: Relation A): Closure Transitive P (TCl P) where
+  sub := SubRel.mk TCl.inclusion
+  pred := Transitive.mk TCl.trans
+  least := by
+    intros Q sub inst
+    apply SubRel.mk
+    intros a b H
+    induction H
+    case inclusion Hab =>
+      apply P.inclusion
+      apply Hab
+    case trans Hab Hbc =>
+      apply Q.trans
+      apply Hab
+      apply Hbc
+
+
+instance {A: Type}: ClosureOp Transitive (TCl (A := A)) where
+  close := TCl.close
+
+
+instance {A} {P: Relation A}: Transitive (TCl P) where
+  trans := TCl.trans
+
+
+instance {A} {P: Relation A} [Reflexive P]: Reflexive (TCl P) where
+  refl {a} := by
+    apply TCl.inclusion
+    apply P.refl
+
+instance {A} {P: Relation A} [Transitive P]: Transitive (RCl P) where
+  trans {a b c} H1 H2 := by
+    cases H1
+    case inclusion Hab =>
+      cases H2
+      case inclusion Hbc =>
+        apply P.inclusion
+        apply P.trans Hab Hbc
+      case refl =>
+        apply RCl.inclusion
+        apply Hab
+    case refl =>
+      apply H2
+
+instance {A} {P: Relation A}: KeepCong P (TCl P) where
+  keep_cong := by
+    intros f HP a b HC
+    induction HC with
+    | @inclusion a b H =>
+      apply TCl.inclusion (HP H)
+    | @trans a b c Hab Hac IHab IHac =>
+      apply TCl.trans IHab IHac
+
+/--
+`Reflexive` and `Transitive` predicate
+-/
+def RTPred {A: Type}: RelationPred A := fun (P: Relation A) => Reflexive P ∧ Transitive P
+
+/--
+`Reflexive` and `Transitive` Closure
+-/
+inductive RTCl {A} (P: Relation A): Relation A where
+  | inclusion {a b}: P a b -> RTCl P a b
+  | refl {a}: RTCl P a a
+  | trans {a b c}: RTCl P a b -> RTCl P b c -> RTCl P a c
+
+
+instance RTCl.close {A} (P: Relation A): Closure RTPred P (RTCl P) where
+  sub := SubRel.mk RTCl.inclusion
+  pred := by
+    constructor
+    . apply Reflexive.mk
+      apply RTCl.refl
+    . apply Transitive.mk
+      apply RTCl.trans
+  least := by
+    intros Q inst sub
+    let inst_refl := inst.left
+    let inst_trans := inst.right
+    apply SubRel.mk
+    intros a b H
+    induction H
+    case inclusion Hab => apply P.inclusion Hab
+    case refl => apply Q.refl
+    case trans Hab Hbc => apply Q.trans Hab Hbc
+
+
+instance rt_cl_op {A: Type}: ClosureOp RTPred (RTCl (A := A)) where
+  close := RTCl.close
+
+
+instance {A} {P: Relation A}: Reflexive (RTCl P) where
+  refl := RTCl.refl
+
+instance {A} {P: Relation A}: Transitive (RTCl P) where
+  trans := RTCl.trans
+
+
+instance {A} {P: Relation A}: KeepCong P (RTCl P) where
+  keep_cong := by
+    intros f HP a b HC
+    induction HC with
+    | @inclusion a b H =>
+      apply RTCl.inclusion (HP H)
+    | @refl =>
+      apply RTCl.refl
+    | @trans a b c Hab Hac IHab IHac =>
+      apply RTCl.trans IHab IHac
+
+
+/-!
+Then we prove the equivalence between RTCl P, RCl (TCl P) and TCl (RCl P)
+-/
+abbrev RTCl2 {A} (P: Relation A) := RCl (TCl P)
+
+instance RTCl2.close {A} (P: Relation A): Closure RTPred P (RTCl2 P) where
+  sub := by
+    apply SubRel.mk
+    intros a b H
+    apply (TCl P).inclusion
+    apply P.inclusion
+    apply H
+  pred := by
+    constructor
+    . /- Reflexive -/
+      apply Reflexive.mk
+      intros a
+      apply Relation.refl
+    . /- Transitive -/
+      apply Transitive.mk
+      intros a b c
+      apply Relation.trans
+  least := by
+    intros Q inst sub
+    let inst_refl := inst.left
+    let inst_trans := inst.right
+    apply (RCl.close (TCl P)).least inst_refl
+    apply (TCl.close P).least inst_trans
+    exact sub
+
+
+instance rt2_cl_op {A: Type}: ClosureOp RTPred (RTCl2 (A := A)) where
+  close := RTCl2.close
+
+theorem rt2_eq_rt: @RTCl2 = @RTCl := by
+  apply funext
+  intros A
+  let H := @cl_op_unique A RTPred RTCl2 RTCl rt2_cl_op rt_cl_op
+  apply H
+
+
+abbrev RTCl3 {A} (P: Relation A) := TCl (RCl P)
+
+instance RTCl3.close {A} (P: Relation A): Closure RTPred P (RTCl3 P) where
+  sub := by
+    apply SubRel.mk
+    intros a b H
+    apply (TCl P).inclusion
+    apply P.inclusion
+    apply H
+  pred := by
+    constructor
+    . /- Reflexive -/
+      apply Reflexive.mk
+      intros a
+      apply (TCl (RCl P)).refl
+    . /- Transitive -/
+      apply Transitive.mk
+      intros a b c
+      apply (TCl (RCl P)).trans
+  least := by
+    intros Q inst sub
+    let inst_refl := inst.left
+    let inst_trans := inst.right
+    apply (TCl.close (RCl P)).least inst_trans
+    apply (RCl.close P).least inst_refl
+    exact sub
+
+
+instance rt3_cl_op {A: Type}: ClosureOp RTPred (RTCl3 (A := A)) where
+  close := RTCl3.close
+
+theorem rt3_eq_rt: @RTCl3 = @RTCl := by
+  apply funext
+  intros A
+  let H := @cl_op_unique A RTPred RTCl3 RTCl rt3_cl_op rt_cl_op
+  apply H
+
+
+/--
+Symmetric closure
+-/
+inductive SCl {A} (P: Relation A): Relation A where
+  | inclusion {a b}: P a b -> SCl P a b
+  | symm {a b}: SCl P a b -> SCl P b a
+
+instance {A: Type} {P: Relation A}: P sub_rel SCl P where
+  inclusion := SCl.inclusion
+
+instance {A} {P: Relation A}: Symmetric (SCl P) where
+  symm := SCl.symm
+
+instance {A} {P R: Relation A} [P sub_rel R] [Symmetric R]: SCl P sub_rel R where
+  inclusion {a b} H := by
+    induction H
+    case inclusion Hab =>
+      apply P.inclusion
+      apply Hab
+    case symm Hab =>
+      apply R.symm
+      apply Hab
+
+theorem scl_ab_or_ba {A} {P: Relation A}: forall {a b: A}, SCl P a b -> P a b ∨ P b a := by
+  intros a b H
+  induction H
+  case inclusion a b Hab =>
+    left; apply Hab
+  case symm a b H IHH =>
+    cases IHH
+    case inl Hab =>
+      right; apply Hab
+    case inr Hba =>
+      left; apply Hba
+
+
+instance SCl.close {A: Type} (P: Relation A): Closure Symmetric P (SCl P) where
+  sub := SubRel.mk SCl.inclusion
+  pred := Symmetric.mk SCl.symm
+  least := by
+    intros Q sub symm
+    apply SubRel.mk
+    intros a b H
+    have Hab_Hba := scl_ab_or_ba H
+    cases Hab_Hba
+    case inl Hab =>
+      apply P.inclusion
+      exact Hab
+    case inr Hba =>
+      apply Q.symm
+      apply P.inclusion
+      apply Hba
+
+instance {A: Type}: ClosureOp Symmetric SCl (A := A) where
+  close := SCl.close
+
+
+instance {A} {P: Relation A}: Symmetric (SCl P) where
+  symm := SCl.symm
+
+
+/-!
+Similarly, we inspect the equational definitions of an equivalence relation.
+-/
+instance sr_refl {A} {P: Relation A} [Reflexive P]: Reflexive (SCl P) where
+  refl {a}:= by
+    apply SCl.inclusion
+    apply P.refl
+
+instance rs_symm {A} {P: Relation A} [Symmetric P]: Symmetric (RCl P) where
+  symm {a b} H := by
+    cases H
+    case inclusion Hab =>
+      apply P.inclusion
+      apply P.symm Hab
+    case refl Hab =>
+      apply (RCl P).refl
+
+instance ts_symm {A} {P: Relation A} [Symmetric P]: Symmetric (TCl P) where
+  symm {a b} H := by
+    induction H
+    case inclusion Hab =>
+      apply P.inclusion
+      apply P.symm Hab
+    case trans a b c _ _ Hba Hcb =>
+      apply (TCl P).trans Hcb Hba
+
+/-!
+The symmetric closure of a transitive relation is not transitive
+Think about a set ${a, b, c}$, and relation ${(a, b), (c, b)}$, which is transitive.
+Then, the symmetric closure is ${(a, b), (b, a), (c, b), (b, c)}$.
+We can find $(a, b)$ and $(b, c)$ in that, but not $(a, c)$.
+-/
+namespace CounterExampleOfTransSymm
+
+inductive Three: Type where
+  | a | b | c
+
+inductive Rel3: Three -> Three -> Prop where
+  | ab: Rel3 .a .b
+  | cb: Rel3 .c .b
+
+theorem rel3_trans: forall {x y z: Three}, Rel3 x y -> Rel3 y z -> Rel3 x z := by
+  intros x y z Hxy Hyz
+  cases Hxy
+  case ab =>
+    cases Hyz
+  case cb =>
+    cases Hyz
+
+
+instance: Transitive Rel3 where
+  trans {x y z} Hxy Hyz := by
+    cases Hxy
+    case ab =>
+      cases Hyz
+    case cb =>
+      cases Hyz
+
+
+example: Not (Transitive (SCl Rel3)) := by
+  intros H
+  let Hab := SCl.inclusion Rel3.ab
+  let Hcb := SCl.inclusion Rel3.cb
+  let Hbc := SCl.symm Hcb
+  have H2: SCl Rel3 .a .c := by
+    apply (SCl Rel3).trans Hab Hbc
+  let error := scl_ab_or_ba H2
+  cases error
+  case inl E => cases E
+  case inr E => cases E
+
+end CounterExampleOfTransSymm
+
+
+/-!
+Then, we work on the transitive and symmetric closure
+-/
+def TSPred {A: Type}: RelationPred A := fun (P: Relation A) => Transitive P ∧ Symmetric P
+abbrev TSCl {A: Type} (P: Relation A) := TCl (SCl P)
+
+instance TSCl.close {A: Type} (P: Relation A): Closure TSPred P (TSCl P) where
+  sub := by
+    let s1 := (TCl.close (SCl P)).sub
+    let s2 := (SCl.close P).sub
+    apply Relation.trans s2 s1
+  pred := by
+    constructor
+    . /- Transitive -/
+      apply (TCl.close (SCl P)).pred
+    . /- Symmetric -/
+      apply ts_symm
+  least := by
+    intros Q H sub
+    let inst_trans := H.left
+    let inst_symm := H.right
+    apply (TCl.close (SCl P)).least inst_trans
+    apply (SCl.close P).least inst_symm
+    exact sub
+
+/-!
+Then, the equivalence relation
+-/
+def EPred {A: Type} (P: Relation A) := Reflexive P ∧ Transitive P ∧ Symmetric P
+
+/--
+Equivalence Closure
+-/
+inductive ECl {A} (P: Relation A): Relation A where
+  | inclusion {a b}: P a b -> ECl P a b
+  | refl {a}: ECl P a a
+  | trans {a b c}: ECl P a b -> ECl P b c -> ECl P a c
+  | symm {a b}: ECl P a b -> ECl P b a
+
+
+instance ECl.close {A} (P: Relation A): Closure EPred P (ECl P) where
+  sub := SubRel.mk ECl.inclusion
+  pred := by
+    constructor
+    . /- Reflexive -/
+      apply Reflexive.mk ECl.refl
+    constructor
+    . /- Transitive -/
+      apply Transitive.mk ECl.trans
+    . /- Symmetric -/
+      apply Symmetric.mk ECl.symm
+  least := by
+    intros Q inst sub
+    let inst_refl := inst.left
+    let inst_trans := inst.right.left
+    let inst_symm := inst.right.right
+    apply SubRel.mk
+    intros a b H
+    induction H
+    case inclusion a b Hab =>
+      apply sub.inclusion
+      apply Hab
+    case refl a =>
+      apply Q.refl
+    case trans Hab Hbc =>
+      apply Q.trans Hab Hbc
+    case symm Hab =>
+      apply Q.symm Hab
+
+instance ecl_cl_op {A: Type}: ClosureOp EPred ECl (A := A) where
+  close := ECl.close
+
+
+instance {A: Type} {P: Relation A}: SubRel (RTCl P) (ECl P) where
+  inclusion := by
+    intros a b H
+    induction H with
+    | @inclusion a b r =>
+      apply ECl.inclusion r
+    | @refl x =>
+      apply ECl.refl
+    | @trans a b c r1 r2 IHr1 IHr2 =>
+      apply ECl.trans (b := b) IHr1 IHr2
+
+
+/-!
+Similarly, we inspect the equivalence between different closures.
+-/
+abbrev ECl2 {A} (P: Relation A) := RCl (TCl (SCl P))
+
+instance ECl2.close {A} (P: Relation A): Closure EPred P (ECl2 P) where
+  sub := by
+    apply SubRel.mk
+    intros a b H
+    apply (SCl P).inclusion
+    apply SCl.inclusion
+    apply H
+  pred := by
+    constructor
+    . /- Reflexive -/
+      apply (RCl.close (TCl (SCl P))).pred
+    constructor
+    . /- Transitive -/
+      apply Transitive.mk
+      intros a b c Hab Hbc
+      apply Relation.trans Hab Hbc
+    . /- Symmetric -/
+      apply Symmetric.mk
+      intros a b Hab
+      apply Relation.symm Hab
+  least := by
+    intros Q inst sub
+    let ⟨inst_refl, inst_trans, inst_symm⟩ := inst
+    apply (RCl.close (TCl (SCl P))).least inst_refl
+    apply (TCl.close (SCl P)).least inst_trans
+    apply (SCl.close P).least inst_symm
+    exact sub
+
+
+instance ecl2_cl_op {A: Type}: ClosureOp EPred ECl2 (A := A) where
+  close := ECl2.close
+
+theorem ecl2_eq_ecl: @ECl2 = @ECl := by
+  apply funext
+  intros A
+  let E := @cl_op_unique A EPred ECl2 ECl ecl2_cl_op ecl_cl_op
+  apply E
